Hoare.v
@@ -95,27 +95,19 @@ Module ExAssertions.
 (** Paraphrase the following assertions in English. *)
 
 Definition as1 : Assertion := fun st => st X = 3.
-(* x = 3 *)
-  
 Definition as2 : Assertion := fun st => st X <= st Y.
-(* x := y *)
-
 Definition as3 : Assertion :=
   fun st => st X = 3 \/ st X <= st Y.
-(* x := 3 or x := y *)
-
 Definition as4 : Assertion :=
   fun st => st Z * st Z <= st X /\
             ~ (((S (st Z)) * (S (st Z))) <= st X).
-
 Definition as5 : Assertion := fun st => True.
-(* always true *)
-
 Definition as6 : Assertion := fun st => False.
-(* always false *)
+
+(* FILL IN HERE *)
 
 End ExAssertions.
-
+(** [] *)
 
 (* ####################################################### *)
 (** ** Notation for Assertions *)
@@ -196,31 +188,27 @@ Notation "{{ P }}  c  {{ Q }}" :=
 (** **** Exercise: 1 star, optional (triples)  *)
 (** Paraphrase the following Hoare triples in English.
    1) {{True}} c {{X = 5}}
-      after executing command c, state X = 5
 
    2) {{X = m}} c {{X = m + 5)}}
-      If state X = m, after executing command c, then state X = m + 5
 
    3) {{X <= Y}} c {{Y <= X}}
-      If state X <= state Y initially, after executing command c,
-      state Y <= state X. 
 
    4) {{True}} c {{False}}
-      true state becomes false state after executing command c
 
    5) {{X = m}} 
       c
       {{Y = real_fact m}}.
-      If we start out in a state where the value of X is m,
-      and we execute command c,
-      then we finish in a state where Y = real_fact m.
 
    6) {{True}} 
       c 
       {{(Z * Z) <= m /\ ~ (((S Z) * (S Z)) <= m)}}
-      If state is initially true, after executing command c,
-      z*z <=m and (z^2+2z+1) > m)
+
  *)
+
+
+(** [] *)
+
+
 
 
 
@@ -232,39 +220,26 @@ Notation "{{ P }}  c  {{ Q }}" :=
 (** Which of the following Hoare triples are _valid_ -- i.e., the
     claimed relation between [P], [c], and [Q] is true?
    1) {{True}} X ::= 5 {{X = 5}}
-      Valid
- *)
-
-
-(*
 
    2) {{X = 2}} X ::= X + 1 {{X = 3}}
-      Valid
 
    3) {{True}} X ::= 5; Y ::= 0 {{X = 5}}
-      Valid
 
    4) {{X = 2 /\ X = 3}} X ::= 5 {{X = 0}}
-      invalid
 
    5) {{True}} SKIP {{False}}
-      invalid
 
    6) {{False}} SKIP {{True}}
-      valid
 
    7) {{True}} WHILE True DO SKIP END {{False}}
-      invalid
 
    8) {{X = 0}}
       WHILE X == 0 DO X ::= X + 1 END
       {{X = 1}}
-      valid
 
    9) {{X = 1}}
       WHILE X <> 0 DO X ::= X + 1 END
       {{X = 100}}
-      invalidm does not terminate
 
 *)
 (* FILL IN HERE *)
@@ -282,17 +257,18 @@ Theorem hoare_post_true : forall (P Q : Assertion) c,
   (forall st, Q st) ->
   {{P}} c {{Q}}.
 Proof.
-  intros. unfold hoare_triple. intros. apply H.
-Qed.
-
+  intros P Q c H. unfold hoare_triple.
+  intros st st' Heval HP.
+  apply H.  Qed.
 
 Theorem hoare_pre_false : forall (P Q : Assertion) c,
-  (forall st, ~(P st)) -> {{P}} c {{Q}}.
+  (forall st, ~(P st)) ->
+  {{P}} c {{Q}}.
 Proof.
-  intros. unfold hoare_triple. intros. unfold not in H. apply H in H1. inversion H1.
-Qed.
-
-
+  intros P Q c H. unfold hoare_triple.
+  intros st st' Heval HP.
+  unfold not in H. apply H in HP.
+  inversion HP.  Qed.
 
 (* ####################################################### *) 
 (** ** Proof Rules *)
@@ -423,15 +399,10 @@ Notation "P [ X |-> a ]" := (assn_sub X a P) (at level 10).
 Theorem hoare_asgn : forall Q X a,
   {{Q [X |-> a]}} (X ::= a) {{Q}}.
 Proof.
-  intros. unfold hoare_triple. intros. inversion H. unfold assn_sub in H0.
-  rewrite <- H5. assumption.
-Qed.
-(*                
   unfold hoare_triple.
   intros Q X a st st' HE HQ.
   inversion HE. subst.
   unfold assn_sub in HQ. assumption.  Qed.
-*)
 
 (** Here's a first formal proof using this rule. *)
 
@@ -440,8 +411,7 @@ Example assn_sub_example :
   (X ::= (ANum 3))
   {{fun st => st X = 3}}.
 Proof.
-  apply hoare_asgn.
-Qed.
+  apply hoare_asgn.  Qed.
 
 (** **** Exercise: 2 stars (hoare_asgn_examples)  *)
 (** Translate these informal Hoare triples...
@@ -455,24 +425,8 @@ Qed.
    ...into formal statements [assn_sub_ex1, assn_sub_ex2] 
    and use [hoare_asgn] to prove them. *)
 
-Example assn_sub_ex1 :
-   {{(fun st => st X <= 5) [X |-> APlus (AId X)  (ANum 1)] }}
-   X ::= APlus (AId X) (ANum 1)
-   {{fun st => st X <= 5 }}.
-Proof.
-  apply hoare_asgn.
-Qed.
-
-Example assn_sub_ex2:
-  {{(fun st => 0 <= st X /\ st X <= 5) [X |-> (ANum 3)] }}
-  X ::= (ANum 3)
-  {{fun st => 0 <= st X /\ st X <= 5 }}.
-Proof.
-  apply hoare_asgn.
-Qed.
-  
-
-  
+(* FILL IN HERE *)
+(** [] *)
 
 (** **** Exercise: 2 stars (hoare_asgn_wrong)  *)
 (** The assignment rule looks backward to almost everyone the first
@@ -486,24 +440,8 @@ Qed.
     arithmetic expression [a], and your counterexample needs to
     exhibit an [a] for which the rule doesn't work. *)
 
-Example hoare_asgn_wrong_0:
-  {{fun st => True}}
-  X ::= (ANum 1)
-  {{fun st => st X = 1}}.
-Proof.
-  admit.
-
-Example hoare_asgn_wrong:
-  {{fun st => True}}
-  X ::= APlus (AId X) (ANum 1)
-  {{fun st => st X = st X + 1}}.
-Proof.
-  unfold hoare_triple. intros. inversion H.
-  admit.
-Qed.
-
-  
-    
+(* FILL IN HERE *)
+(** [] *)
 
 (** **** Exercise: 3 stars, advanced (hoare_asgn_fwd)  *)
 (** However, using an auxiliary variable [m] to remember the original
@@ -530,8 +468,8 @@ Theorem hoare_asgn_fwd :
   {{fun st => P (update st X m) /\ st X = aeval (update st X m) a }}.
 Proof.
   intros functional_extensionality m a P.
- admit. 
-   
+  (* FILL IN HERE *) Admitted.
+(** [] *)
 
 (** **** Exercise: 2 stars, advanced (hoare_asgn_fwd_exists)  *)
 (** Another way to define a forward rule for assignment is to
@@ -555,14 +493,9 @@ Theorem hoare_asgn_fwd_exists :
                 st X = aeval (update st X m) a }}.
 Proof.
   intros functional_extensionality a P.
-  unfold hoare_triple.
-  intros.
-  inversion H.
-  rewrite -> H4.
-  exists n.
-  split.
-admit.
-  
+  (* FILL IN HERE *) Admitted.
+(** [] *)
+
 (* ####################################################### *) 
 (** *** Consequence *)
 
@@ -609,19 +542,20 @@ Theorem hoare_consequence_pre : forall (P P' Q : Assertion) c,
   P ->> P' ->
   {{P}} c {{Q}}.
 Proof.
-  intros. intros st st' Hc HP. apply (H st st'). assumption. apply H0. assumption.
-Qed.
+  intros P P' Q c Hhoare Himp.
+  intros st st' Hc HP. apply (Hhoare st st'). 
+  assumption. apply Himp. assumption. Qed.
 
 Theorem hoare_consequence_post : forall (P Q Q' : Assertion) c,
   {{P}} c {{Q'}} ->
   Q' ->> Q ->
   {{P}} c {{Q}}.
 Proof.
-  intros. intros st st' Hc HP. apply H0. apply (H st st'). assumption. assumption.
-Qed.
-
-
-
+  intros P Q Q' c Hhoare Himp.
+  intros st st' Hc HP. 
+  apply Himp.
+  apply (Hhoare st st'). 
+  assumption. assumption. Qed.
 
 (** For example, we might use the first consequence rule like this:
                 {{ True }} ->>
@@ -635,12 +569,10 @@ Example hoare_asgn_example1 :
   {{fun st => True}} (X ::= (ANum 1)) {{fun st => st X = 1}}.
 Proof.
   apply hoare_consequence_pre
-  with (P' := (fun st => st X = 1) [X |-> (ANum 1)]).
-  apply hoare_asgn. intros st H. unfold assn_sub. simpl. reflexivity.
+    with (P' := (fun st => st X = 1) [X |-> ANum 1]).
+  apply hoare_asgn.
+  intros st H. unfold assn_sub, update. simpl. reflexivity.
 Qed.
-
-
-
 
 (** Finally, for convenience in some proofs, we can state a "combined"
     rule of consequence that allows us to vary both the precondition
@@ -658,14 +590,10 @@ Theorem hoare_consequence : forall (P P' Q Q' : Assertion) c,
   Q' ->> Q ->
   {{P}} c {{Q}}.
 Proof.
-  intros. apply hoare_consequence_pre with (P' := P').
+  intros P P' Q Q' c Hht HPP' HQ'Q.
+  apply hoare_consequence_pre with (P' := P').
   apply hoare_consequence_post with (Q' := Q').
-  apply H.
-  assumption. assumption.
-Qed.
-                                               
-  
-
+  assumption. assumption. assumption.  Qed.
 
 (* ####################################################### *)
 (** *** Digression: The [eapply] Tactic *)
@@ -694,8 +622,7 @@ Example hoare_asgn_example1' :
 Proof.
   eapply hoare_consequence_pre.
   apply hoare_asgn.
-  intros st H.  reflexivity.
-Qed.
+  intros st H.  reflexivity.  Qed.
 
 (** In general, [eapply H] tactic works just like [apply H] except
     that, instead of failing if unifying the goal with the conclusion
@@ -741,7 +668,8 @@ Abort.
     instantiated with terms containing (ordinary) variables that did
     not exist at the time the existential variable was created. *)
 
-Lemma silly2 : forall (P : nat -> nat -> Prop) (Q : nat -> Prop),
+Lemma silly2 :
+  forall (P : nat -> nat -> Prop) (Q : nat -> Prop),
   (exists y, P 42 y) ->
   (forall x y : nat, P x y -> Q x) ->
   Q 42.
@@ -755,7 +683,8 @@ Proof.
 
 Abort.
 
-Lemma silly2_fixed : forall (P : nat -> nat -> Prop) (Q : nat -> Prop),
+Lemma silly2_fixed :
+  forall (P : nat -> nat -> Prop) (Q : nat -> Prop),
   (exists y, P 42 y) ->
   (forall x y : nat, P x y -> Q x) ->
   Q 42.
@@ -789,32 +718,8 @@ Qed.
    ...into formal statements [assn_sub_ex1', assn_sub_ex2'] and 
    use [hoare_asgn] and [hoare_consequence_pre] to prove them. *)
 
-Example assn_sub_ex1' :
-  {{fun st => st X + 1 <= 5 }}
-  X ::= (APlus (AId X) (ANum 1))
-  {{fun st => st X <= 5 }}.
-Proof.
-  eapply hoare_consequence_pre. eapply hoare_asgn.
-  intros st H. unfold assn_sub, update. destruct (eq_id_dec X X).
-  apply H.
-  unfold not in n. apply ex_falso_quodlibet. apply n. reflexivity.
-Qed.
-
-
-Example assn_sub_ex2' :
-  {{fun st => 0 <= 3 /\ 3 <= 5 }}
-  X ::= (ANum 3)
-  {{fun st => 0 <= st X /\ st X <= 5 }}.
-Proof.
-  eapply hoare_consequence_pre. eapply hoare_asgn.
-  intros st H. unfold assn_sub, update.
-  destruct (eq_id_dec X X).
-  simpl. assumption.
-  unfold not in n. apply ex_falso_quodlibet. apply n. reflexivity.
-Qed.
-  
-
-
+(* FILL IN HERE *)
+(** [] *)
 
 (* ####################################################### *)
 (** *** Skip *)
@@ -850,12 +755,10 @@ Theorem hoare_seq : forall P Q R c1 c2,
      {{P}} c1 {{Q}} ->
      {{P}} c1;;c2 {{R}}.
 Proof.
-  intros P Q R c1 c2. intros H1 H2.  intros st st' Hc Pre.
-  inversion Hc. subst.
-  apply (H1 st'0 st').  assumption.
-  apply (H2 st st'0). assumption.
-  assumption.
-Qed.
+  intros P Q R c1 c2 H1 H2 st st' H12 Pre.
+  inversion H12; subst.
+  apply (H1 st'0 st'); try assumption.
+  apply (H2 st st'0); assumption. Qed.
 
 (** Note that, in the formal rule [hoare_seq], the premises are
     given in "backwards" order ([c2] before [c1]).  This matches the
@@ -880,15 +783,12 @@ Example hoare_asgn_example3 : forall a n,
   (X ::= a;; SKIP) 
   {{fun st => st X = n}}.
 Proof.
-  intros.
-  eapply hoare_seq.
-  Case "right". eapply hoare_skip.
-  Case "left". eapply hoare_consequence_pre. apply hoare_asgn.
-  intros st H. subst. reflexivity.
-Qed.
-
-
-
+  intros a n. eapply hoare_seq.
+  Case "right part of seq".
+    apply hoare_skip.
+  Case "left part of seq".
+    eapply hoare_consequence_pre. apply hoare_asgn. 
+    intros st H. subst. reflexivity. Qed.
 
 (** You will most often use [hoare_seq] and
     [hoare_consequence_pre] in conjunction with the [eapply] tactic,
@@ -903,19 +803,14 @@ Qed.
                    {{ X = 1 /\ 2 = 2 }}
     Y ::= 2
                    {{ X = 1 /\ Y = 2 }}
- *)
+*)
 
 Example hoare_asgn_example4 :
   {{fun st => True}} (X ::= (ANum 1);; Y ::= (ANum 2)) 
   {{fun st => st X = 1 /\ st Y = 2}}.
 Proof.
-  eapply hoare_seq.
-  Case "first". apply hoare_asgn.
-  Case "second". eapply hoare_consequence_pre.
-  eapply hoare_asgn.
-  intros st H. subst.
-Abort.
-
+  (* FILL IN HERE *) Admitted.
+(** [] *)
 
 (** **** Exercise: 3 stars (swap_exercise)  *)
 (** Write an Imp program [c] that swaps the values of [X] and [Y]
@@ -925,22 +820,15 @@ Abort.
 *)
 
 Definition swap_program : com :=
-  Z ::= (AId X);; X ::= (AId Y) ;; Y ::= (AId Z).
+  (* FILL IN HERE *) admit.
 
 Theorem swap_exercise :
   {{fun st => st X <= st Y}} 
   swap_program
   {{fun st => st Y <= st X}}.
 Proof.
-  unfold swap_program.
-  eapply hoare_seq. eapply hoare_seq.
-  Case "first". apply hoare_asgn.
-  Case "second". apply hoare_asgn.
-  Case "third".
-  eapply hoare_consequence_pre.
-  eapply hoare_asgn.
-  intros st H.  apply H.
-Qed.
+  (* FILL IN HERE *) Admitted.
+(** [] *)
 
 (** **** Exercise: 3 stars (hoarestate1)  *)
 (** Explain why the following proposition can't be proven:
